Update adequacy theorems for RustLang and RustHalt

nola/examples/rust_halt/adequacy.v
@@ -1,8 +1,28 @@
 (** * Adequacy *)
 
+From nola.rust_lang Require Export adequacy.
 From nola.examples.rust_halt Require Export type num.
 
 Implicit Type JUDG : ofe.
+
+(** Ghost state *)
+Class rust_haltGpreS CON Σ : Type := RustHaltGpreS {
+  rust_haltGpreS_lrust :: lrustGpreS Σ;
+  rust_haltGoreS_inv :: inv'GpreS (cifOF CON) Σ;
+  rust_haltGpreS_na_inv :: na_invG Σ;
+  rust_haltGpreS_dinv :: dinvGpreS (cifOF CON) Σ;
+  rust_haltGpreS_token :: tokenG Σ;
+  rust_haltGpreS_borrow :: borrowGpreS (cifOF CON) Σ;
+  rust_haltGpreS_proph :: prophGpreS xty Σ;
+  rust_haltGpreS_proph_ag :: proph_agG nat xty Σ;
+  rust_haltGpreS_fborrow :: fborrowGpreS (cifOF CON) Σ;
+}.
+Definition rust_haltΣ CON : gFunctors :=
+  #[lrustΣ; inv'Σ (cifOF CON); na_invΣ; dinvΣ (cifOF CON); tokenΣ;
+    borrowΣ (cifOF CON); prophΣ xty; proph_agΣ nat xty; fborrowΣ (cifOF CON)].
+Global Instance subG_rust_haltGpreS `{!subG (rust_haltΣ CON) Σ} :
+  rust_haltGpreS CON Σ.
+Proof. solve_inG. Qed.
 
 (** Allocate the world satisfaction *)
 Lemma rust_wsat_alloc `{!rust_haltGpreS CON Σ,
@@ -20,30 +40,30 @@ Proof.
   iApply "Wfborrow".
 Qed.
 
-(** Usual adequacy for a partial weakest precondition *)
-Theorem wp_adequacy `{!rust_haltGpreS CON Σ} {JUDG e σ φ} :
+(** Safety adequacy for a partial weakest precondition *)
+Theorem wp_adequacy `{!rust_haltGpreS CON Σ} {JUDG s e σ φ} :
   (∀ `{!rust_haltGS CON Σ}, ∃ (_ : Csem CON JUDG Σ) (_ : Jsem JUDG (iProp Σ)),
-    ⊢ |={⊤}=> WP[rust_halt_wsat] e {{ v, |=[rust_halt_wsat]{⊤}=> ⌜φ v⌝ }}) →
-  adequate NotStuck e σ (λ v _, φ v).
+    own heap_name (◯ to_heap σ) ={⊤}=∗ WP[rust_halt_wsat] e @ s; ⊤ {{ v, ∀ σ',
+      own heap_name (● to_heap σ') -∗ rust_halt_wsat ={⊤,∅}=∗ ⌜φ v σ'⌝ }}) →
+  adequate s e σ φ.
 Proof.
-  move=> towp. eapply lrust_adequacy; [exact _|]=> ?.
+  move=> towp. eapply lrust_adequacy=> ?. iIntros "◯σ".
   iMod rust_wsat_alloc as (?<-) "→W". case: (towp _)=> ?[? wp].
-  iMod wp as "wp". rewrite wpw_fupdw_fupdw. iDestruct ("→W" $! _ _) as "W".
-  iExists _. by iMod ("wp" with "W") as "[? $]".
+  iMod (wp with "◯σ") as "$". iModIntro. iApply "→W".
 Qed.
 
-(** Termination adequacy over a total weakest precondition *)
-Theorem twp_total `{!rust_haltGpreS CON Σ} {JUDG e σ} :
+(** Termination adequacy for a total weakest precondition *)
+Theorem twp_total `{!rust_haltGpreS CON Σ} {JUDG s e σ} :
   (∀ `{!rust_haltGS CON Σ}, ∃ (_ : Csem CON JUDG Σ) (_ : Jsem JUDG (iProp Σ)) Φ,
-    ⊢ |={⊤}=> WP[rust_halt_wsat] e [{ Φ }]) →
+    own heap_name (◯ to_heap σ) ={⊤}=∗ WP[rust_halt_wsat] e @ s; ⊤ [{ Φ }]) →
   sn erased_step ([e], σ).
 Proof.
-  move=> totwp. eapply lrust_total; [exact _|]=> ?.
+  move=> totwp. eapply lrust_total=> ?. iIntros "◯σ".
   iMod rust_wsat_alloc as (?<-) "→W". case: (totwp _)=> ?[?[? twp]].
-  iMod twp as "$". iModIntro. iApply "→W".
+  iMod (twp with "◯σ") as "$". iModIntro. iApply "→W".
 Qed.
 
-(** Usual adequacy over a typing judgment *)
+(** Safety adequacy for a typing judgment *)
 Theorem type_adeqaucy `{!rust_haltGpreS CON Σ} {Xl post pre Γo e σ JUDG} :
   pre post () →
   (∀ `{!rust_haltGS CON Σ}, ∃ (_ : Csem CON JUDG Σ) (_ : Jsem JUDG (iProp Σ)),
@@ -51,13 +71,14 @@ Theorem type_adeqaucy `{!rust_haltGpreS CON Σ} {Xl post pre Γo e σ JUDG} :
   adequate NotStuck e σ (λ _ _, ∃ xl, post xl).
 Proof.
   move=> topre totyp. eapply wp_adequacy=> ?. case: (totyp _)=> ?[? typ].
-  exists _, _. rewrite type_unseal in typ.
+  exists _, _. iIntros "_". rewrite type_unseal in typ.
   iMod (na_alloc (na_invG0:=rust_haltGS_na_inv)) as (t) "t". iModIntro.
-  iDestruct (typ $! 1%Qp t (λ _, post) (λ _,()) with "[//] t [] [//]")
+  iDestruct (typ $! 1%Qp t (λ _, post) (λ _, ()) with "[//] t [] [//]")
     as "twp".
   { by iApply proph_obs_true. }
-  iApply twp_wp. iApply (twp_mono with "twp")=> ?. f_equiv.
-  iDestruct 1 as "(% & _ & _ & obs & _)". rewrite proph_obs_sat.
+  iApply twp_wp. iApply (twp_mono with "twp")=> ?. iIntros "to" (?) "_ W".
+  iMod ("to" with "W") as "[_(% & _ & _ & obs & _)]".
+  iApply fupd_mask_intro_discard; [done|]. rewrite proph_obs_sat.
   iDestruct "obs" as "[% %]". by iExists _.
 Qed.
 Theorem type_adeqaucy_int `{!rust_haltGpreS CON Σ, !rust_haltC CON}
@@ -68,19 +89,20 @@ Theorem type_adeqaucy_int `{!rust_haltGpreS CON Σ, !rust_haltC CON}
   adequate NotStuck e σ (λ v _, ∃ (n : Z) xl, v = #n ∧ post (n ᵖ:: xl)).
 Proof.
   move=> topre totyp. eapply wp_adequacy=> ?. case: (totyp _)=> ?[? typ].
-  exists _, _. rewrite type_unseal in typ.
+  exists _, _. iIntros "_". rewrite type_unseal in typ.
   iMod (na_alloc (na_invG0:=rust_haltGS_na_inv)) as (t) "t". iModIntro.
-  iDestruct (typ $! 1%Qp t (λ _, post) (λ _,()) with "[//] t [] [//]")
+  iDestruct (typ $! 1%Qp t (λ _, post) (λ _, ()) with "[//] t [] [//]")
     as "twp".
   { by iApply proph_obs_true. }
-  iApply twp_wp. iApply (twp_mono with "twp")=> ?. f_equiv.
-  rewrite /ty_int ty_pty_unseal /=. iDestruct 1 as "(% & _ & _ & obs & %i & _)".
-  case i=> [?[? +]]. rewrite of_path_val. move=> [[->][?[eq[->]]]].
-  rewrite proph_obs_sat. iDestruct "obs" as "[%π %]". rewrite -(eq π).
-  by iExists _, _.
+  iApply twp_wp. iApply (twp_mono with "twp")=> ?. iIntros "to" (?) "_ W".
+  rewrite /ty_int ty_pty_unseal /=.
+  iMod ("to" with "W") as "[_(% & _ & _ & obs & %i & _)]".
+  iApply fupd_mask_intro_discard; [done|]. case i=> [?[? +]].
+  rewrite of_path_val. move=> [[->][?[eq[->]]]]. rewrite proph_obs_sat.
+  iDestruct "obs" as "[%π %]". rewrite -(eq π). by iExists _, _.
 Qed.
 
-(** Termination adequacy over a typing judgment *)
+(** Termination adequacy for a typing judgment *)
 Theorem type_total `{!rust_haltGpreS CON Σ} {Xl post pre Γo e σ JUDG} :
   pre post () →
   (∀ `{!rust_haltGS CON Σ}, ∃ (_ : Csem CON JUDG Σ) (_ : Jsem JUDG (iProp Σ)),
@@ -88,9 +110,9 @@ Theorem type_total `{!rust_haltGpreS CON Σ} {Xl post pre Γo e σ JUDG} :
   sn erased_step ([e], σ).
 Proof.
   move=> topre totyp. eapply twp_total=> ?. case: (totyp _)=> ?[? typ].
-  exists _, _, (λ _, True)%I. rewrite type_unseal in typ.
+  exists _, _, (λ _, True)%I. iIntros "_". rewrite type_unseal in typ.
   iMod (na_alloc (na_invG0:=rust_haltGS_na_inv)) as (t) "t". iModIntro.
-  iDestruct (typ $! 1%Qp t (λ _, post) (λ _,()) with "[//] t [] [//]")
+  iDestruct (typ $! 1%Qp t (λ _, post) (λ _, ()) with "[//] t [] [//]")
     as "twp"; [by iApply proph_obs_true|].
   iApply (twp_mono with "twp"). by iIntros.
 Qed.
