nola/rust_lang/adequacy.v
@@ -21,39 +21,42 @@ Global Instance subG_lrustGpreS {Σ} : subG lrustΣ Σ → lrustGpreS Σ.
 Proof. solve_inG. Qed.
 
 (** Partial correctness adequacy *)
-Theorem lrust_adequacy Σ `{!lrustGpreS Σ} hlc e σ φ :
-  (∀ `{!lrustGS_gen hlc Σ}, ⊢ |={⊤}=>
-    ∃ W : iProp Σ, W ∗ WP[W] e {{ v, ⌜φ v⌝ }}) →
-  adequate NotStuck e σ (λ v _, φ v).
+Theorem lrust_adequacy `{!lrustGpreS Σ} {hlc s e σ φ} :
+  (∀ `{!lrustGS_gen hlc Σ}, own heap_name (◯ to_heap σ) ={⊤}=∗
+    ∃ W : iProp Σ, W ∗ WP[W] e @ s; ⊤ {{ v,
+      ∀ σ', own heap_name (● to_heap σ') -∗ W ={⊤,∅}=∗ ⌜φ v σ'⌝ }}) →
+  adequate s e σ φ.
 Proof.
   move=> big. apply adequate_alt=> ?? /erased_steps_nsteps[?[??]].
   eapply (wpw_strong_adequacy_gen hlc Σ _); [|done]=> Hinv.
-  iMod (own_alloc (● to_heap σ)) as (vγ) "?".
-  { apply (auth_auth_valid (to_heap _)), to_heap_valid. }
+  iMod (own_alloc (● to_heap σ ⋅ ◯ to_heap σ)) as (vγ) "[? ◯σ]".
+  { apply auth_both_valid. split=>//. exact: to_heap_valid. }
   iMod (own_alloc (● (∅ : heap_freeableUR))) as (fγ) "?";
     first by apply auth_auth_valid.
   set Hheap := HeapGS _ _ _ vγ fγ.
-  iMod (big (LRustGS _ _ Hinv Hheap)) as (W) "[??]". iModIntro.
+  iMod (big (LRustGS _ _ Hinv Hheap) with "◯σ") as (W) "[??]". iModIntro.
   iExists _, [_], _, _, _=>/=. iFrame. iSplit; [done|].
-  iIntros (??->??) "_ _ H _". iApply fupd_mask_intro_discard; [done|].
-  iSplit; [|done].
-  iDestruct (big_sepL2_cons_inv_r with "H") as (?? ->) "[? H]".
-  iDestruct (big_sepL2_nil_inv_r with "H") as %->. iIntros (??[=-><-]).
-  by rewrite to_of_val.
+  iIntros (??->??) "W [%[●σ' _]] H _".
+  iDestruct (big_sepL2_cons_inv_r with "H") as (e' ? ->) "[→φ H]".
+  iDestruct (big_sepL2_nil_inv_r with "H") as %->=>/=. case eq: (to_val e')=>/=.
+  - iMod ("→φ" with "●σ' W") as %?. iModIntro. iSplit; [|done].
+    iIntros (??[=-><-]). move: eq. rewrite to_of_val=> [[->]]. by iPureIntro.
+  - iApply fupd_mask_intro_discard; [done|]. iSplit; [|done]. iPureIntro.
+    move=> ??[??]. subst. move: eq. by rewrite to_of_val.
 Qed.
 
 (** Termination adequacy *)
-Theorem lrust_total Σ `{!lrustGpreS Σ} s e σ :
-  (∀ `{!lrustGS_gen HasNoLc Σ}, ⊢ |={⊤}=>
+Theorem lrust_total `{!lrustGpreS Σ} {s e σ} :
+  (∀ `{!lrustGS_gen HasNoLc Σ}, own heap_name (◯ to_heap σ) ={⊤}=∗
     ∃ W Φ, W ∗ WP[W] e @ s; ⊤ [{ Φ }]) →
   sn erased_step ([e], σ).
 Proof.
   move=> big. eapply (twpw_total _ _ _ _ _ 0)=> Hinv.
-  iMod (own_alloc (● to_heap σ)) as (vγ) "?".
-  { apply (auth_auth_valid (to_heap _)), to_heap_valid. }
+  iMod (own_alloc (● to_heap σ ⋅ ◯ to_heap σ)) as (vγ) "[? ◯σ]".
+  { apply auth_both_valid. split=>//. exact: to_heap_valid. }
   iMod (own_alloc (● (∅ : heap_freeableUR))) as (fγ) "?";
     first by apply auth_auth_valid.
   set Hheap := HeapGS _ _ _ vγ fγ.
-  iMod (big (LRustGS _ _ Hinv Hheap)) as (??) "[??]". iModIntro.
+  iMod (big (LRustGS _ _ Hinv Hheap) with "◯σ") as (??) "[??]". iModIntro.
   iExists _, _, _, _, _. by iFrame.
 Qed.
